\clarification[4]{In the second part of the exercise we also need to assume that $A$ is a symmetric $n\times n$ matrix.}

\noindent We have
\begin{align*}
    \transpose{(A^{-1})} &= (\transpose{A})^{-1} \\
    &= A^{-1},
\end{align*}
so $A^{-1}$ is symmetric.

In the second part, since $A$ is symmetric,
\begin{align*}
    \transpose{(BA\transpose{B})} &= \transpose{(\transpose{B})}\transpose{A}\transpose{B} \\
    &= BA\transpose{B},
\end{align*}
so the product $BA\transpose{B}$ gives a symmetric matrix.
